ProofLibrary/TermBasics.lean
@@ -13,6 +13,7 @@ structure SkolemFS (sig : Signature) [DecidableEq sig.V] where
   ruleId : Nat
   disjunctIndex : Nat
   var : sig.V
+  arity : Nat -- NOTE: this is not enforced anywhere; we set this when skolemizing to remember the frontier size
   deriving DecidableEq
 
 abbrev GroundTerm (sig : Signature) [DecidableEq sig.C] [DecidableEq sig.V] := FiniteTree (SkolemFS sig) sig.C
@@ -148,7 +149,7 @@ namespace VarOrConst
     match voc with
       | .var v => ite (v ∈ frontier)
         (SkolemTerm.var v)
-        (SkolemTerm.func { ruleId, disjunctIndex, var := v} frontier)
+        (SkolemTerm.func { ruleId, disjunctIndex, var := v, arity := frontier.length } frontier)
       | .const c => SkolemTerm.const c
 
   theorem skolemize_injective (ruleId : Nat) (disjunctIndex : Nat) (frontier : List sig.V) (s t : VarOrConst sig) : s.skolemize ruleId disjunctIndex frontier = t.skolemize ruleId disjunctIndex frontier -> s = t := by
@@ -229,5 +230,206 @@ section ListsOfTerms
                 apply h.right
                 simp [t_mem]
             . rfl
+
+  def all_terms_limited_by_depth (constants : List sig.C) (funcs : List (SkolemFS sig)) : Nat -> List (GroundTerm sig)
+  | 0 => []
+  | 1 => constants.map GroundTerm.const
+  | .succ (.succ depth) =>
+    let prev := all_terms_limited_by_depth constants funcs (.succ depth)
+    funcs.flatMap (fun func =>
+      (all_term_lists_of_length prev func.arity).map (fun ts =>
+        FiniteTree.inner func (FiniteTreeList.fromList ts)
+      )
+    )
+
+  theorem mem_all_terms_limited_by_depth (constants : List sig.C) (funcs : List (SkolemFS sig)) (depth : Nat) :
+      ∀ t, t ∈ (all_terms_limited_by_depth constants funcs depth) ↔ (t.depth ≤ depth ∧ (∀ c, c ∈ t.leaves -> c ∈ constants) ∧ (∀ func, func ∈ t.innerLabels -> func ∈ funcs)) := by
+    induction depth with
+    | zero =>
+      simp [all_terms_limited_by_depth]
+      intro t t_depth
+      cases t <;> simp [FiniteTree.depth] at t_depth
+    | succ depth ih =>
+      intro t
+      unfold all_terms_limited_by_depth
+
+      cases t with
+      | leaf c => sorry
+      | inner t_func ts =>
+
+        cases depth with
+        | zero =>
+          simp only [Nat.zero_add]
+          sorry
+        | succ depth =>
+          simp only [List.mem_flatMap, List.mem_map]
+
+          let rec aux : ∀ (ts : FiniteTreeList (SkolemFS sig) sig.C), (∀ t, t ∈ ts.toList -> t ∈ (all_terms_limited_by_depth constants funcs depth.succ)) ↔
+              ((FiniteTree.depthList ts ≤ depth.succ) ∧ (∀ c, c ∈ FiniteTree.leavesList ts -> c ∈ constants) ∧ (∀ func, func ∈ FiniteTree.innerLabelsList ts -> func ∈ funcs)) := by
+            intro ts
+            cases ts with
+            | nil =>
+              simp [FiniteTree.depthList, FiniteTree.leavesList, FiniteTree.innerLabelsList, FiniteTreeList.toList]
+            | cons hd tl =>
+              unfold FiniteTree.depthList
+              unfold FiniteTree.leavesList
+              unfold FiniteTree.innerLabelsList
+
+              specialize ih hd
+              have ih_inner := aux tl
+
+              constructor
+              . intro h
+
+                have ih := ih.mp (by
+                  apply h
+                  unfold FiniteTreeList.toList
+                  simp
+                )
+                have ih_inner := ih_inner.mp (by
+                  intro t t_mem
+                  apply h
+                  unfold FiniteTreeList.toList
+                  simp [t_mem]
+                )
+
+                constructor
+                . rw [Nat.max_le]
+                  constructor
+                  . apply ih.left
+                  . apply ih_inner.left
+                constructor
+                . intro c c_mem
+                  rw [List.mem_append] at c_mem
+                  cases c_mem with
+                  | inl c_mem => apply ih.right.left; exact c_mem
+                  | inr c_mem => apply ih_inner.right.left; exact c_mem
+                . intro func func_mem
+                  rw [List.mem_append] at func_mem
+                  cases func_mem with
+                  | inl func_mem => apply ih.right.right; exact func_mem
+                  | inr func_mem => apply ih_inner.right.right; exact func_mem
+              . intro h
+
+                have ih := ih.mpr (by
+                  sorry
+                  /- apply h -/
+                  /- unfold FiniteTreeList.toList -/
+                  /- simp -/
+                )
+                have ih_inner := ih_inner.mpr (by
+                  sorry
+                  /- intro t t_mem -/
+                  /- apply h -/
+                  /- unfold FiniteTreeList.toList -/
+                  /- simp [t_mem] -/
+                )
+                intro t t_mem
+                unfold FiniteTreeList.toList at t_mem
+                rw [List.mem_cons] at t_mem
+                cases t_mem with
+                | inl t_mem => rw [t_mem]; apply ih
+                | inr t_mem => apply ih_inner; exact t_mem
+
+          constructor
+          . intro h
+            rcases h with ⟨func, func_mem, ts, ts_mem, t_eq⟩
+            rw [← t_eq]
+            rw [mem_all_term_lists_of_length] at ts_mem
+
+            /- let rec aux : ∀ (ts : FiniteTreeList (SkolemFS sig) sig.C), (∀ t, t ∈ ts.toList -> t ∈ (all_terms_limited_by_depth constants funcs depth.succ)) -> -/
+            /-     ((FiniteTree.depthList ts ≤ depth.succ) ∧ (∀ c, c ∈ FiniteTree.leavesList ts -> c ∈ constants) ∧ (∀ func, func ∈ FiniteTree.innerLabelsList ts -> func ∈ funcs)) := by -/
+            /-   intro ts -/
+            /-   cases ts with -/
+            /-   | nil => -/
+            /-     intro h -/
+            /-     constructor -/
+            /-     . simp [FiniteTree.depthList] -/
+            /-     constructor -/
+            /-     . simp [FiniteTree.leavesList] -/
+            /-     . simp [FiniteTree.innerLabelsList] -/
+            /-   | cons hd tl => -/
+            /-     intro h -/
+            /-     unfold FiniteTree.depthList -/
+            /-     unfold FiniteTree.leavesList -/
+            /-     unfold FiniteTree.innerLabelsList -/
+            /-     specialize ih hd -/
+            /-     have ih := ih.mp (by -/
+            /-       apply h -/
+            /-       unfold FiniteTreeList.toList -/
+            /-       simp -/
+            /-     ) -/
+            /-     have ih_inner := aux tl (by -/
+            /-       intro t t_mem -/
+            /-       apply h -/
+            /-       unfold FiniteTreeList.toList -/
+            /-       simp [t_mem] -/
+            /-     ) -/
+            /-     constructor -/
+            /-     . rw [Nat.max_le] -/
+            /-       constructor -/
+            /-       . apply ih.left -/
+            /-       . apply ih_inner.left -/
+            /-     constructor -/
+            /-     . intro c c_mem -/
+            /-       rw [List.mem_append] at c_mem -/
+            /-       cases c_mem with -/
+            /-       | inl c_mem => apply ih.right.left; exact c_mem -/
+            /-       | inr c_mem => apply ih_inner.right.left; exact c_mem -/
+            /-     . intro func func_mem -/
+            /-       rw [List.mem_append] at func_mem -/
+            /-       cases func_mem with -/
+            /-       | inl func_mem => apply ih.right.right; exact func_mem -/
+            /-       | inr func_mem => apply ih_inner.right.right; exact func_mem -/
+
+            unfold FiniteTree.depth
+            unfold FiniteTree.leaves
+            unfold FiniteTree.innerLabels
+
+            have this := (aux (FiniteTreeList.fromList ts)).mp (by intro t t_mem; rw [FiniteTreeList.fromListToListIsId] at t_mem; apply ts_mem.right; exact t_mem)
+            constructor
+            . rw [Nat.add_comm]
+              apply Nat.succ_le_succ
+              exact this.left
+            constructor
+            . exact this.right.left
+            . intro func' func'_mem
+              rw [List.mem_cons] at func'_mem
+              cases func'_mem with
+              | inl func'_mem => rw [func'_mem]; exact func_mem
+              | inr func'_mem => apply this.right.right; exact func'_mem
+
+          . intro h
+            exists t_func
+            constructor
+            . apply h.right.right
+              unfold FiniteTree.innerLabels
+              simp
+            exists ts
+
+            unfold FiniteTree.depth at h
+            unfold FiniteTree.leaves at h
+            unfold FiniteTree.innerLabels at h
+
+            have this := (aux ts).mpr (by
+              constructor
+              . rw [Nat.add_comm] at h
+                rw [Nat.succ_le_succ_iff] at h
+                exact h.left
+              constructor
+              . exact h.right.left
+              . intro func func_mem
+                apply h.right.right
+                simp [func_mem]
+            )
+
+            constructor
+            . rw [mem_all_term_lists_of_length]
+              constructor
+              . sorry
+              . intro t t_mem
+                apply this
+                exact t_mem
+            . rw [FiniteTreeList.toListFromListIsId]
 
 end ListsOfTerms
